To condense the expression $3 \ln 3 - \frac{1}{2} \ln(x^2 + 1)$, we apply the following properties of logarithms:

1.  **Power Property**: $n \ln a = \ln(a^n)$
2.  **Difference Property**: $\ln a - \ln b = \ln\left(\frac{a}{b}\right)$

### Step-by-Step Solution:

1.  **Apply the Power Property to each term:**
    *   First term: $3 \ln 3 = \ln(3^3) = \ln 27$
    *   Second term: $\frac{1}{2} \ln(x^2 + 1) = \ln((x^2 + 1)^{1/2}) = \ln(\sqrt{x^2 + 1})$

2.  **Rewrite the expression:**
    $$\ln 27 - \ln(\sqrt{x^2 + 1})$$

3.  **Apply the Difference Property:**
    $$\ln\left(\frac{27}{\sqrt{x^2 + 1}}\right)$$

**Final Answer:**
$$\ln\left(\frac{27}{\sqrt{x^2 + 1}}\right)$$